language/move-prover/bytecode-to-boogie/tests/goldenfiles/libra_account.bpl
@@ -374,7 +374,8 @@ ensures old(b#Boolean(Boolean(!(b#Boolean(ExistsResource(m, LibraCoin_MarketCap_
 
     // assume arguments are of correct types
     assume is#Integer(arg0);
-    assume IsValidReferenceParameter(local_counter, arg1);
+    assume is#Vector(Dereference(m, arg1));
+    assume IsValidReferenceParameter(m, local_counter, arg1);
 
     old_size := local_counter;
     local_counter := local_counter + 24;
@@ -672,7 +673,8 @@ ensures b#Boolean(Boolean((ret0) == (SelectField(Dereference(m, arg0), LibraCoin
     saved_m := m;
 
     // assume arguments are of correct types
-    assume IsValidReferenceParameter(local_counter, arg0);
+    assume is#Vector(Dereference(m, arg0));
+    assume IsValidReferenceParameter(m, local_counter, arg0);
 
     old_size := local_counter;
     local_counter := local_counter + 4;
@@ -803,7 +805,8 @@ ensures old(b#Boolean(Boolean(i#Integer(SelectField(Dereference(m, arg0), LibraC
     saved_m := m;
 
     // assume arguments are of correct types
-    assume IsValidReferenceParameter(local_counter, arg0);
+    assume is#Vector(Dereference(m, arg0));
+    assume IsValidReferenceParameter(m, local_counter, arg0);
     assume is#Integer(arg1);
 
     old_size := local_counter;
@@ -968,7 +971,8 @@ ensures old(b#Boolean(Boolean(i#Integer(Integer(i#Integer(SelectField(Dereferenc
     saved_m := m;
 
     // assume arguments are of correct types
-    assume IsValidReferenceParameter(local_counter, arg0);
+    assume is#Vector(Dereference(m, arg0));
+    assume IsValidReferenceParameter(m, local_counter, arg0);
     assume is#Vector(arg1);
 
     old_size := local_counter;
@@ -1675,7 +1679,8 @@ ensures old(b#Boolean(Boolean(i#Integer(SelectField(SelectField(Dereference(m, a
     saved_m := m;
 
     // assume arguments are of correct types
-    assume IsValidReferenceParameter(local_counter, arg0);
+    assume is#Vector(Dereference(m, arg0));
+    assume IsValidReferenceParameter(m, local_counter, arg0);
     assume is#Integer(arg1);
 
     old_size := local_counter;
@@ -1830,7 +1835,8 @@ ensures old(b#Boolean(Boolean(!(b#Boolean(ExistsResource(m, LibraAccount_T_type_
     saved_m := m;
 
     // assume arguments are of correct types
-    assume IsValidReferenceParameter(local_counter, arg0);
+    assume is#Vector(Dereference(m, arg0));
+    assume IsValidReferenceParameter(m, local_counter, arg0);
     assume is#Integer(arg1);
 
     old_size := local_counter;
@@ -2076,7 +2082,8 @@ requires ExistsTxnSenderAccount(m, txn);
 
     // assume arguments are of correct types
     assume is#Address(arg0);
-    assume IsValidReferenceParameter(local_counter, arg1);
+    assume is#Vector(Dereference(m, arg1));
+    assume IsValidReferenceParameter(m, local_counter, arg1);
     assume is#Integer(arg2);
     assume is#ByteArray(arg3);
 
@@ -2299,7 +2306,8 @@ requires ExistsTxnSenderAccount(m, txn);
     saved_m := m;
 
     // assume arguments are of correct types
-    assume IsValidReferenceParameter(local_counter, arg0);
+    assume is#Vector(Dereference(m, arg0));
+    assume IsValidReferenceParameter(m, local_counter, arg0);
     assume is#ByteArray(arg1);
 
     old_size := local_counter;
@@ -2425,7 +2433,8 @@ requires ExistsTxnSenderAccount(m, txn);
     saved_m := m;
 
     // assume arguments are of correct types
-    assume IsValidReferenceParameter(local_counter, arg0);
+    assume is#Vector(Dereference(m, arg0));
+    assume IsValidReferenceParameter(m, local_counter, arg0);
     assume is#ByteArray(arg1);
 
     old_size := local_counter;
@@ -2851,7 +2860,8 @@ requires ExistsTxnSenderAccount(m, txn);
     saved_m := m;
 
     // assume arguments are of correct types
-    assume IsValidReferenceParameter(local_counter, arg0);
+    assume is#Vector(Dereference(m, arg0));
+    assume IsValidReferenceParameter(m, local_counter, arg0);
 
     old_size := local_counter;
     local_counter := local_counter + 6;
@@ -2955,7 +2965,8 @@ requires ExistsTxnSenderAccount(m, txn);
     saved_m := m;
 
     // assume arguments are of correct types
-    assume IsValidReferenceParameter(local_counter, arg0);
+    assume is#Vector(Dereference(m, arg0));
+    assume IsValidReferenceParameter(m, local_counter, arg0);
 
     old_size := local_counter;
     local_counter := local_counter + 4;
@@ -3155,7 +3166,8 @@ requires ExistsTxnSenderAccount(m, txn);
     saved_m := m;
 
     // assume arguments are of correct types
-    assume IsValidReferenceParameter(local_counter, arg0);
+    assume is#Vector(Dereference(m, arg0));
+    assume IsValidReferenceParameter(m, local_counter, arg0);
 
     old_size := local_counter;
     local_counter := local_counter + 3;
@@ -3196,7 +3208,8 @@ requires ExistsTxnSenderAccount(m, txn);
     saved_m := m;
 
     // assume arguments are of correct types
-    assume IsValidReferenceParameter(local_counter, arg0);
+    assume is#Vector(Dereference(m, arg0));
+    assume IsValidReferenceParameter(m, local_counter, arg0);
 
     old_size := local_counter;
     local_counter := local_counter + 3;
@@ -3740,7 +3753,8 @@ requires ExistsTxnSenderAccount(m, txn);
     saved_m := m;
 
     // assume arguments are of correct types
-    assume IsValidReferenceParameter(local_counter, arg0);
+    assume is#Vector(Dereference(m, arg0));
+    assume IsValidReferenceParameter(m, local_counter, arg0);
     assume is#Address(arg1);
 
     old_size := local_counter;
@@ -3853,7 +3867,8 @@ requires ExistsTxnSenderAccount(m, txn);
     saved_m := m;
 
     // assume arguments are of correct types
-    assume IsValidReferenceParameter(local_counter, arg0);
+    assume is#Vector(Dereference(m, arg0));
+    assume IsValidReferenceParameter(m, local_counter, arg0);
     assume is#Address(arg1);
 
     old_size := local_counter;
@@ -3989,7 +4004,8 @@ requires ExistsTxnSenderAccount(m, txn);
     saved_m := m;
 
     // assume arguments are of correct types
-    assume IsValidReferenceParameter(local_counter, arg0);
+    assume is#Vector(Dereference(m, arg0));
+    assume IsValidReferenceParameter(m, local_counter, arg0);
 
     old_size := local_counter;
     local_counter := local_counter + 18;
