language/move-prover/bytecode-to-boogie/tests/goldenfiles/verify-local-ref.bpl
@@ -22,7 +22,8 @@ requires ExistsTxnSenderAccount(m, txn);
     saved_m := m;
 
     // assume arguments are of correct types
-    assume IsValidReferenceParameter(local_counter, arg0);
+    assume is#Integer(Dereference(m, arg0));
+    assume IsValidReferenceParameter(m, local_counter, arg0);
 
     old_size := local_counter;
     local_counter := local_counter + 3;
